\documentclass[12pt]{article}

\usepackage[top=1in,bottom=1.5in,left=1in,right=1in]{geometry}
\usepackage{amsmath,bbm}
\allowdisplaybreaks
\usepackage[colorlinks=true,allcolors=magenta]{hyperref}

\begin{document}
\setlength{\parskip}{3mm}
\setlength{\parindent}{7mm}

\section{Exponential model}

The differential equation is
%
\begin{equation}
  c'(s) = r c(s)\,,
\end{equation}
%
and can be rewritten as
%
\begin{equation}
  \label{eq:exponential-integrand}
  \frac{1}{c(s)} c'(s) = r\,.
\end{equation}
%
Integrating \eqref{eq:exponential-integrand} from $s = 0$ to $s = t$:
%
\begin{equation}
  \log|c(t)| - \log|c(0)|
  = \log\bigg|\frac{c(t)}{c(0)}\bigg|
  = \log\bigg(\frac{c(t)}{c(0)}\bigg)
  = rt\,.
\end{equation}
%
Solving for $c(t)$:
%
\begin{equation}
  \label{eq:exponential}
  c(t) = c(0) e^{r t}\,.
\end{equation}


\section{Subexponential model}

The differential equation is
%
\begin{equation}
  c'(s) = \alpha c(s)^p\,,\qquad p \in (0,1)\,,
\end{equation}
%
and can be rewritten as
%
\begin{equation}
  \label{eq:subexponential-integrand}
  \frac{1}{c(s)^p} c'(s) = \alpha\,.
\end{equation}
%
Integrating \eqref{eq:subexponential-integrand} from $s = 0$ to $s = t$:
%
\begin{equation}
  \frac{1}{1 - p} \big[c(t)^{1 - p} - c(0)^{1 - p}\big] = \alpha t\,.
\end{equation}
%
Solving for $c(t)$:
%
\begin{equation}
  \label{eq:subexponential}
  c(t) = \big[c(0)^{1 - p} + (1 - p) \alpha t\big]^{1 / (1 - p)}\,.
\end{equation}


\section{Gompertz model}

The differential equation is
%
\begin{equation}
  c'(t) = \alpha c(t) \log \bigg(\frac{K}{c(t)}\bigg)\,,
\end{equation}
%
with solution
%
\begin{equation}
  \label{eq:gompertz}
  c(t) = K \bigg(\frac{c(0)}{K}\bigg)^{e^{-\alpha t}}\,.
\end{equation}


\section{Logistic model}

The differential equation is
%
\begin{equation}
  c'(s) = r c(s) \bigg(1 - \frac{c(s)}{K}\bigg)\,,
\end{equation}
%
and can be rewritten as
%
\begin{equation}
  \label{eq:logistic-integrand}
  \bigg(\frac{1}{c(s) - K} - \frac{1}{c(s)}\bigg) c'(s) = -r\,.
\end{equation}
%
Integrating \eqref{eq:logistic-integrand} from $s = 0$ to $s = t$:
%
\begin{equation}
  \begin{aligned}
    &\log|c(t) - K| - \log|c(t)| - \log|c(0) - K| + \log|c(0)| \\
    &= \log\bigg|\frac{c(0) (c(t) - K)}{c(t) (c(0) - K)}\bigg| \\
    &= \log\bigg(\frac{c(0) (c(t) - K)}{c(t) (c(0) - K)}\bigg) \\
    &= -rt\,.
  \end{aligned}
\end{equation}
%
Solving for $c(t)$:
%
\begin{equation}
  \label{eq:logistic}
  c(t) = \frac{K}{1 + \big(\frac{K}{c(0)} - 1\big) e^{-r t}}\,.
\end{equation}

\subsection{Reparametrization}

$c''(t_\text{infl}) = 0$ reduces to
%
\begin{equation}
  \label{eq:logistic-tinfl}
  \frac{K}{c(0)} - 1 = e^{r t_\text{infl}}\,.
\end{equation}
%
Substituting \eqref{eq:logistic-tinfl} in \eqref{eq:logistic}:
%
\begin{equation}
  c(t) = \frac{K}{1 + e^{-r (t - t_\text{infl})}}\,.
\end{equation}

\section{Richards model}

The differential equation is
%
\begin{equation}
  c'(s) = r c(s) \bigg(1 - \bigg(\frac{c(s)}{K}\bigg)^a\bigg)\,,
\end{equation}
%
and can be rewritten as
%
\begin{equation}
  \label{eq:richards-integrand}
  \bigg(\frac{1}{c(s) (c(s)^a - K^a)}\bigg) c'(s) = -\frac{r}{K^a}\,.
\end{equation}
%
One can verify that
%
\begin{equation}
  \int \frac{1}{x (x^a - b^a)}\,\text{d}x = \frac{1}{a b^a} \log\bigg|\frac{b^a}{x^a} - 1\bigg|\,.
\end{equation}
%
Integrating \eqref{eq:richards-integrand} from $s = 0$ to $s = t$:
%
\begin{equation}
  \begin{aligned}
    &\frac{1}{a K^a} \Bigg(\log\bigg|\frac{K^a}{c(t)^a} - 1\bigg| - \log\bigg|\frac{K^a}{c(0)^a} - 1\bigg|\Bigg) \\
    &= \frac{1}{a K^a} \log\Bigg|\frac{\frac{K^a}{c(t)^a} - 1}{\frac{K^a}{c(0)^a} - 1}\Bigg| \\
    &= \frac{1}{a K^a} \log\Bigg(\frac{\frac{K^a}{c(t)^a} - 1}{\frac{K^a}{c(0)^a} - 1}\Bigg) \\
    &= -\frac{r}{K^a}t\,.
  \end{aligned}
\end{equation}
%
Solving for $c(t)$:
%
\begin{equation}
  \label{eq:richards}
  c(t) = \frac{K}{\big[1 + \big(\big(\frac{K}{c(0)}\big)^a - 1\big) e^{-r a t}\big]^{1/a}}\,.
\end{equation}

\subsection{Reparametrization}

$c''(t_\text{infl}) = 0$ reduces to
%
\begin{equation}
  \label{eq:richards-tinfl}
  \bigg(\frac{K}{c(0)}\bigg)^a - 1 = a e^{r a t_\text{infl}}\,.
\end{equation}
%
Substituting \eqref{eq:richards-tinfl} in \eqref{eq:richards}:
%
\begin{equation}
  c(t) = \frac{K}{\big[1 + a e^{-r a (t - t_\text{infl})}\big]^{1/a}}\,.
\end{equation}


\end{document}
