\documentclass[12pt]{article}

\usepackage[top=1in,bottom=1.5in,left=1in,right=1in]{geometry}
\usepackage{amsmath,bbm}
\allowdisplaybreaks
\usepackage[colorlinks=true,allcolors=magenta]{hyperref}

\begin{document}
\setlength{\parskip}{3mm}
\setlength{\parindent}{7mm}

\section{Logistic model}

The differential equation is
%
\begin{equation}
  x'(s) = r x(s) \bigg(1 - \frac{x(s)}{K}\bigg)\,,
\end{equation}
%
and can be rewritten as
%
\begin{equation}
  \label{eq:logistic-integrand}
  \bigg(\frac{1}{x(s) - K} - \frac{1}{x(s)}\bigg) x'(s) = -r\,.
\end{equation}
%
Integrating \eqref{eq:logistic-integrand} from $s = 0$ to $s = t$:
%
\begin{equation}
  \begin{aligned}
    &\log|x(t) - K| - \log|x(t)| - \log|x(0) - K| + \log|x(0)| \\
    &= \log\bigg|\frac{x(0) (x(t) - K)}{x(t) (x(0) - K)}\bigg| \\
    &= \log\bigg(\frac{x(0) (x(t) - K)}{x(t) (x(0) - K)}\bigg) \\
    &= -rt\,.
  \end{aligned}
\end{equation}
%
Solving for $x(t)$:
%
\begin{equation}
  \label{eq:logistic}
  x(t) = \frac{K}{1 + \big(\frac{K}{x(0)} - 1\big) e^{-r t}}\,.
\end{equation}

\subsection{Reparametrization}

Solving $x(t_\text{half}) = \frac{K}{2}$ for $\frac{K}{x(0)}$:
%
\begin{equation}
  \label{eq:logistic-thalf}
  \frac{K}{2} = \frac{K}{1 + \big(\frac{K}{x(0)} - 1\big) e^{-r t_\text{half}}}
  \implies \frac{K}{x(0)} = e^{r t_\text{half}} + 1\,.
\end{equation}
%
Substituting \eqref{eq:logistic-thalf} in \eqref{eq:logistic}:
%
\begin{equation}
  x(t) = \frac{K}{1 + e^{-r (t - t_\text{half})}}\,.
\end{equation}

\section{Richards model}

The differential equation is
%
\begin{equation}
  x'(s) = r x(s) \bigg(1 - \bigg(\frac{x(s)}{K}\bigg)^p\bigg)\,,
\end{equation}
%
and can be rewritten as
%
\begin{equation}
  \label{eq:richards-integrand}
  \bigg(\frac{1}{x(s) (x(s)^p - K^p)}\bigg) x'(s) = -\frac{r}{K^p}\,.
\end{equation}
%
One can verify that
%
\begin{equation}
  \int \frac{1}{x (x^p - K^p)}\,\text{d}x = \frac{1}{p K^p} \log\bigg|\frac{K^p}{x^p} - 1\bigg|\,.
\end{equation}
%
Integrating \eqref{eq:richards-integrand} from $s = 0$ to $s = t$:
%
\begin{equation}
  \begin{aligned}
    &\frac{1}{p K^p} \Bigg(\log\bigg|\frac{K^p}{x(t)^p} - 1\bigg| - \log\bigg|\frac{K^p}{x(0)^p} - 1\bigg|\Bigg) \\
    &= \frac{1}{p K^p} \log\Bigg|\frac{\frac{K^p}{x(t)^p} - 1}{\frac{K^p}{x(0)^p} - 1}\Bigg| \\
    &= \frac{1}{p K^p} \log\Bigg(\frac{\frac{K^p}{x(t)^p} - 1}{\frac{K^p}{x(0)^p} - 1}\Bigg) \\
    &= -\frac{r}{K^p}t\,.
  \end{aligned}
\end{equation}
%
Solving for $x(t)$:
%
\begin{equation}
  \label{eq:richards}
  x(t) = \frac{K}{\big[1 + \big(\big(\frac{K}{x(0)}\big)^p - 1\big) e^{-r p t}\big]^{1/p}}\,.
\end{equation}

\subsection{Reparametrization}

Solving $x(t_\text{half}) = \frac{K}{2}$ for $\big(\frac{K}{x(0)}\big)^p$:
%
\begin{equation}
  \label{eq:richards-thalf}
  \frac{K}{2} = \frac{K}{\big[1 + \big(\big(\frac{K}{x(0)}\big)^p - 1\big) e^{-r p t_\text{half}}\big]^{1/p}} \implies \bigg(\frac{K}{x(0)}\bigg)^p = 1 + (2^p - 1) e^{r p t_\text{half}}\,.
\end{equation}
%
Substituting \eqref{eq:richards-thalf} in \eqref{eq:richards}:
%
\begin{equation}
  x(t) = \frac{K}{\big[1 + (2^p - 1) e^{-r p (t - t_\text{half})}\big]^{1/p}}\,.
\end{equation}

\end{document}
